specs/old/Spec.Old.Ed25519.fst
@@ -150,8 +150,6 @@ let sign (secret:lbytes 32) (msg:bytes{length msg < pow2 32 - 64}) =
   let s = (r + ((h * (little_endian a)) % q)) % q in
   rs @| little_bytes 32ul s
 
-let sign_test secret msg = sign secret msg
-
 let sign_expanded (ks:lbytes 96) (msg:bytes{length msg < pow2 32 - 64}) =
   let a, prefix = Seq.slice ks 32 64, Seq.slice ks 64 96 in
   let a' = Seq.slice ks 0 32 in
